Some borken proofs were reconstructed, a few left to resolve

CheckerProofScript.sml
@@ -1,7 +1,8 @@
 open preamble CheckerSpecTheory CheckerTheory
-  
+open ratTheory
+
 val _ = new_theory "CheckerProof";
-   
+      
 val EWIN_thm = Q.store_thm("EWIN_thm",
   `EWIN = EWIN_dec`,
   simp[FUN_EQ_THM]
@@ -22,7 +23,7 @@ val HWIN_thm = Q.store_thm("HWIN_thm",
   \\ PairCases_on`p`
   \\ rw[HWIN_def,HWIN_dec_def]
   \\ metis_tac[HWIN_def,HWIN_dec_def])
- 
+  
 val GET_CAND_TALLY_HEAD_REMOVAL_def = Q.store_thm ("GET_CAND_TALLY_HEAD_REM",
 `!(h: cand #rat) t c. (~(c = FST h)) ==> (get_cand_tally c (h::t) = get_cand_tally c t)`,
           Induct_on `t `
@@ -125,7 +126,7 @@ val non_empty_IS_CORRECT = Q.store_thm ("non_empty_IS_CORRECT",
             >- rw [non_empty]
             >- rw[non_empty]);
 
-*)
+*) 
  
 
 
@@ -239,7 +240,7 @@ val NoDupCand_BOTH_SIDES= Q.store_thm ("NoDupCand_BOTH_SIDES",
                >-   (rfs[CONS_11]
                     >> first_assum (qspecl_then [`l2`,`c`,`t`,`h2`] strip_assume_tac)
                       >> rfs[])));
- 
+  
 
 
 
@@ -330,7 +331,7 @@ val LogicalLessThanQu_IMP_less_than_quota =Q.store_thm ("LogicalLessThanQu_IMP_l
                    >> metis_tac [])
         >- (`less_than_quota qu t h` by  metis_tac[MEM]
            >> fs[less_than_quota_def])))
-              
+               
  
 val bigger_than_cand_OK = Q.store_thm ("bigger_than_cand_OK",
  `!c t h. (bigger_than_cand c t h) ==> (!d. (MEM d h) ==> (get_cand_tally c t <= get_cand_tally d t))`,
@@ -390,7 +391,7 @@ val Logical_bigger_than_cand_IMP_TheFunctional = Q.store_thm ("Logical_bigger_th
                        >> RW_TAC bool_ss []) 
              >-( first_assum(qspecl_then [`t`,`c`] strip_assume_tac) 
                >> rfs[bigger_than_cand_def,MEM])));
-  
+   
 
  
 val SUBPILE_ONE_HEAD_REMOVAL = Q.store_thm ("SUBPILE_ONE_HEAD_REMOVAL",
@@ -460,7 +461,7 @@ val EVERY_CAND_HAS_ONE_PILE = Q.store_thm ("EVERY_CAND_HAS_ONE_PILE",
       
 
 
-
+ 
 
      
 val Logical_subpile1_IMP_TheFunctional = Q.store_thm ("Logical_subpile1_IMP_TheFunctional",
@@ -602,36 +603,37 @@ val Elim_cand_dec_def = Define `
                /\ (MEM (c,[]) p')
                /\ (subpile1 c p p') /\ (subpile2 c p' p) )) `;
 *)
- 
- 
+  
+(* to be reconstructed
+
 val Logical_elim_to_Functional_Elim = Q.store_thm ("Logical_elim_to_Functional_Elim",
  `!st qu l c j1 j2. ELIM_CAND c (qu,st,l) j1 j2 ==> (ELIM_CAND_dec c (qu,st,l) j1 j2)`,
 
    (rw[ELIM_CAND_def,ELIM_CAND_dec_def]  
     >> EVAL_TAC  
      >> REPEAT STRIP_TAC)  
-      >- rw[]  
-      >- RW_TAC bool_ss []  
+      >- rw[]     
+      >- RW_TAC bool_ss []     
       >- (`l <> []` by metis_tac[Valid_Init_CandList_def]
          >> `?l1 x. l = x::l1` by metis_tac [list_nchotomy]
            >> fs[NULL])
       >- fs[Valid_Init_CandList_def]  
-   
-
->- (`!(l1:cand list) l2 (c':cand). MEM c' l1 \/ MEM c' l2 ==> MEM c' (l1++l2)`
+      >- (`!(l1:cand list) l2 (c':cand). MEM c' l1 \/ MEM c' l2 ==> MEM c' (l1++l2)`
               by FULL_SIMP_TAC list_ss [MEM,MEM_APPEND]
           >> `!c'. MEM c' (h++e) ==> MEM c' l` by metis_tac [MEM,MEM_APPEND]
             >> metis_tac [Logical_list_MEM_VICE_VERCA_TheFunctional])   
-      >- metis_tac [NO_DUP_PRED_to_no_dup]
-      >- metis_tac [PileTally_to_PileTally_DEC1,Valid_PileTally]
-      >- metis_tac [PileTally_to_PileTally_DEC2,Valid_PileTally]
-      >- metis_tac [PileTally_to_PileTally_DEC1,Valid_PileTally]
-      >- metis_tac [PileTally_to_PileTally_DEC2,Valid_PileTally]
-      >- metis_tac [NO_DUP_PRED_to_no_dup]
-      >- metis_tac [Valid_PileTally,PileTally_to_PileTally_DEC1]
-      >- metis_tac [Valid_PileTally,PileTally_to_PileTally_DEC2]
+      >- rw[]        
+      >- metis_tac [PileTally_to_PileTally_DEC1,Valid_PileTally_def]       
+      >- metis_tac [PileTally_to_PileTally_DEC2,Valid_PileTally_def] 
+      >- metis_tac [PileTally_to_PileTally_DEC1,Valid_PileTally_def] 
+      >- metis_tac [PileTally_to_PileTally_DEC2,Valid_PileTally_def]  
       >- rw []
-      >- metis_tac [LogicalLessThanQu_IMP_less_than_quota,Valid_PileTally]
+      >- metis_tac [Valid_PileTally_def,PileTally_to_PileTally_DEC1] 
+      >- metis_tac [Valid_PileTally_def,PileTally_to_PileTally_DEC2]
+      >- rw []
+
+ 
+      >- metis_tac [LogicalLessThanQu_IMP_less_than_quota,Valid_PileTally_def,ALOOKUP_def]
       >- metis_tac [EQE_IMP_REMOVE_ONE_CAND]
       >- (`MEM c (MAP FST t)` by metis_tac [Valid_PileTally,FST,MAP]
         >> `!d. MEM d h ==> MEM d (MAP FST t)` by metis_tac [Valid_PileTally]
@@ -640,32 +642,25 @@ val Logical_elim_to_Functional_Elim = Q.store_thm ("Logical_elim_to_Functional_E
       >- metis_tac [Logical_subpile1_IMP_TheFunctional]
       >- (`!d. (d = c) ==> ?l. MEM (c,l) p` by metis_tac[GET_CAND_PILE_MEM,Valid_PileTally]
           >> metis_tac [Logical_subpile2_IMP_TheFunctional]));
+*)
+ 
 
-
-val empty_list_verified= Q.store_thm ("empty_list_verified",
- `!l. empty_list l ==> (l = [])`,
-
-   Induct_on `l`
-     >- rw[]
-     >- metis_tac[empty_list_def]);
-
-
-
-
-
+(* to be reconstructed
 
 val Functional_Elim_to_Logical_elim = Q.store_thm ("Functional_Elim_to_Logical_elim",
- `!st qu l c j1 j2. Elim_cand_dec st qu l c (j1,j2) ==> elim_cand st qu l c j1 j2`,
+ `!st qu l c j1 j2. ELIM_CAND_dec c (qu,st,l) j1 j2 ==> ELIM_CAND c (qu,st,l) j1 j2`,
+
+
 
   (STRIP_TAC
      >> STRIP_TAC >> STRIP_TAC >> STRIP_TAC >> STRIP_TAC >> STRIP_TAC
-       >> Cases_on `j1`)
-         >- (Cases_on `j2`
-           >- ((rw[Elim_cand_dec_def,elim_cand_def]
+       >> Cases_on `j1`) 
+         >- (Cases_on `j2`   
+           >- ((rw[ELIM_CAND_dec_def,ELIM_CAND_def] 
             >> Cases_on `p` >> Cases_on `r` >> Cases_on `r'` >> Cases_on `r` >> Cases_on `r'`
              >> Cases_on `p'` >> Cases_on `r'` >> Cases_on `r''` >> Cases_on `r'` >> Cases_on `r''`
-              >> rfs[Elim_cand_dec_def]
-               >> REPEAT STRIP_TAC)
+              >>  rfs[ELIM_CAND_def,ELIM_CAND_dec_def]      
+               >> REPEAT STRIP_TAC) 
                 >- metis_tac[empty_list_verified]
                 >- (RW_TAC bool_ss [empty_list_def]
                  >> metis_tac [empty_list_verified])
@@ -727,32 +722,34 @@ val Functional_Elim_to_Logical_elim = Q.store_thm ("Functional_Elim_to_Logical_e
         >- (Cases_on `j2`
             >- RW_TAC bool_ss [Elim_cand_dec_def]
             >- rw[Elim_cand_dec_def]));
+*)
 
 
+(* to be reconstructed
 
 val Logical_transfer_to_Functional_Transfer = Q.store_thm ("Logical_transfer_to_Functional_Transfer",
- `! st qu l j1 j2. transfer st qu l j1 j2 ==> Transfer_dec st qu l (j1,j2)`,
+ `! st qu l j1 j2. TRANSFER (qu,st,l) j1 j2 ==> TRANSFER_dec (qu,st,l) j1 j2`,
 
-(rw[transfer_def,Transfer_dec_def]
+(rw[TRANSFER_def,TRANSFER_dec_def]
   >> EVAL_TAC
     >> REPEAT STRIP_TAC)
-
-     >- rw[]
+ 
+     >- rw[] 
      >- (`(!d. MEM d h \/ MEM d e ==> MEM d l) ==> (!d. MEM d (h++e) ==> MEM d l)`
          by  FULL_SIMP_TAC list_ss [MEM_APPEND] >>
       metis_tac [Logical_list_MEM_VICE_VERCA_TheFunctional])
-     >- metis_tac [NO_DUP_PRED_to_no_dup]
-     >- metis_tac [PileTally_to_PileTally_DEC1,Valid_PileTally]
-     >- metis_tac [PileTally_to_PileTally_DEC2,Valid_PileTally]
-     >- metis_tac [PileTally_to_PileTally_DEC1,Valid_PileTally]
-     >- metis_tac [PileTally_to_PileTally_DEC2,Valid_PileTally]
-     >- metis_tac [PileTally_to_PileTally_DEC1,Valid_PileTally]
-     >- metis_tac [PileTally_to_PileTally_DEC2,Valid_PileTally]
-     >- (`?l1 y. l = y::l1` by metis_tac [Valid_Init_CandList,list_nchotomy]
-         >> rw[non_empty])
-     >- metis_tac [NO_DUP_PRED_to_no_dup,Valid_Init_CandList]
-     >- metis_tac [NO_DUP_PRED_to_no_dup]
-     >- metis_tac [LogicalLessThanQu_IMP_less_than_quota,Valid_PileTally]
+     >- rw[] 
+     >- metis_tac [PileTally_to_PileTally_DEC1,Valid_PileTally_def]
+     >- metis_tac [PileTally_to_PileTally_DEC2,Valid_PileTally_def] 
+     >- metis_tac [PileTally_to_PileTally_DEC1,Valid_PileTally_def] 
+     >- metis_tac [PileTally_to_PileTally_DEC2,Valid_PileTally_def] 
+     >- metis_tac [PileTally_to_PileTally_DEC1,Valid_PileTally_def]
+     >- metis_tac [PileTally_to_PileTally_DEC2,Valid_PileTally_def] 
+     >- (`?l1 y. l = y::l1` by metis_tac [Valid_Init_CandList_def,list_nchotomy]
+         >> fs[NULL])  
+     >- metis_tac [Valid_Init_CandList_def]  
+     >- rw[] 
+     >- metis_tac [LogicalLessThanQu_IMP_less_than_quota,Valid_PileTally_def]
      >- RW_TAC bool_ss []
      >- metis_tac [Logical_subpile1_IMP_TheFunctional]
      >- (`?(y: (Cand # (((Cand list) # rat) list))). (c = FST y) /\ (MEM y np)`
@@ -811,43 +808,43 @@ val Functional_Transfer_to_Logical_transfer = Q.store_thm ("Functional_Transfer_
     >- (Cases_on `j2`
      >- rfs [Transfer_dec_def]
      >- rfs [Transfer_dec_def]));
+*)
 
 
-
-
+  
 val fcc_to_first_continuing_cand = Q.store_thm ("fcc_to_first_continuing_cand",
- `! c b h. fcc c b h ==> first_continuing_cand c b h`,
+ `! c b h. first_continuing_cand_dec c b h ==> first_continuing_cand c b h`,
 
   Induct_on `b`
-    >- rw[fcc_dec]
+    >- rw[first_continuing_cand_dec_def]  
     >- ((REPEAT STRIP_TAC
-      >> rw[first_continuing_cand]
-       >> `(c = h) \/ (~ (c = h))` by metis_tac [CAND_EQ_DEC])
+      >>  rw[first_continuing_cand_def] 
+       >> Cases_on `c = h`) 
          >- (MAP_EVERY qexists_tac [`[]`,`b`]
-          >> FULL_SIMP_TAC list_ss [APPEND_NIL_LEFT])
-         >- (rfs [fcc_dec]
-           >- RW_TAC bool_ss []
-           >- (rfs [first_continuing_cand]
+          >> FULL_SIMP_TAC list_ss [APPEND_NIL_LEFT]) 
+         >- (rfs [first_continuing_cand_dec_def] 
+           >- RW_TAC bool_ss [] 
+           >- (rfs [first_continuing_cand_def]
             >> `?L1 L2. (b = L1 ++ [c]++L2) /\ (!d. MEM d L1 ==> ~ MEM d h')` by metis_tac[]
-             >> MAP_EVERY qexists_tac [`h::L1`,`L2`]
-              >> FULL_SIMP_TAC list_ss [MEM] >> metis_tac [MEM]))));
+             >> MAP_EVERY qexists_tac [`h::L1`,`L2`] 
+              >> FULL_SIMP_TAC list_ss [MEM] >> metis_tac [MEM])))); 
+ 
 
-
-
+ 
 val first_continuing_cand_IMP_fcc = Q.store_thm ("first_continuing_cand_IMP_fcc",
- `! c b h. first_continuing_cand c b h ==> fcc c b h`,
+ `! c b h. first_continuing_cand c b h ==> first_continuing_cand_dec c b h`,
 
 Induct_on `b`
 
->- rw[first_continuing_cand]
+>- rw[first_continuing_cand_def]
 
 >- ((REPEAT STRIP_TAC
-  >> rw[fcc_dec]
-    >> `(c = h) \/ (~ (c = h))` by metis_tac [CAND_EQ_DEC])
+  >> rw[first_continuing_cand_dec_def]
+    >> Cases_on `c = h`)
 
     >- RW_TAC bool_ss []
 
-    >- ((rfs [first_continuing_cand]
+    >- ((rfs [first_continuing_cand_def]
       >> `(l1 = []) \/ (?L1 x. l1 = x::L1)` by metis_tac [list_nchotomy])
 
         >- FULL_SIMP_TAC list_ss [APPEND_NIL_LEFT,CONS_11]
@@ -857,10 +854,10 @@ Induct_on `b`
             >> metis_tac [MEM]))));
 
 
-
+  
 val intermediate_count_def = Define `
-        (intermediate_count st qu l j1 j2 = ? ba t nt p np bl e h.
-          (j1 = state (ba, t, p, bl, e, h))
+        (intermediate_count (qu,st,l) j1 j2 = ? ba t nt p np bl e h.
+          (j1 = NonFinal (ba, t, p, bl, e, h))
        /\ (!d. MEM d (h++e) ==> MEM d l)
        /\ ALL_DISTINCT (h++e)
        /\ (Valid_PileTally t l)
@@ -883,71 +880,22 @@ val intermediate_count_def = Define `
                             /\ (~ MEM c h ==>
                                            (get_cand_pile c np = get_cand_pile c p)
                                         /\ (get_cand_tally c nt = get_cand_tally c t))))
-       /\ (j2 = state ([], nt, np, bl, e, h)))`;
+       /\ (j2 = NonFinal ([], nt, np, bl, e, h)))`;
 
-val COUNT_def = Define `
-         (Count st qu l j1 j2 = ? ba t nt p np bl e h.
-          (j1 = state (ba, t, p, bl, e, h))
-       /\ (!d. MEM d (h++e) ==> MEM d l)
-       /\ (!d. NO_DUP_PRED (h++e) d)
-       /\ (Valid_PileTally t l)
-       /\ (Valid_PileTally nt l)
-       /\ (Valid_PileTally p l)
-       /\ (Valid_PileTally np l)
-       /\ (Valid_Init_CandList l)
-       /\ (!d. NO_DUP_PRED (MAP FST p) d)
-       /\ (!c. NO_DUP_PRED (MAP FST t) c)
-       /\ (!c. NO_DUP_PRED (MAP FST np) c)
-       /\ (!c. NO_DUP_PRED (MAP FST nt) c)
-       /\ (ba <> [])
-       /\ (h <> [])
-       /\ (!c. MEM c l ==>
-                            ((MEM c h ==>
-                             ?(l: ((cand list) # rat) list).
-                               (l = FILTER (\ (b: (cand list) # rat). (first_continuing_cand c (FST b) h)) ba)
-                            /\ (!l'. MEM (c,l') np ==> (l' = (get_cand_pile c p) ++ l))
-                            /\ (!r. MEM (c,r) nt ==> (r = SUM_RAT (MAP SND l))))
-                            /\ (~ MEM c h ==>
-                                           (!l'. MEM c l /\ MEM (c,l') np <=> MEM c l /\ MEM (c,l') p)
-                                        /\ (!r. MEM c l /\ MEM (c,r) t <=> MEM c l /\ MEM (c,r) nt))))
-       /\ (j2 = state ([], nt, np, bl, e, h)))`;
 
 val COUNTAux_dec = Define `
-     (COUNTAux_dec p np t nt ba h [] = T)
-  /\ (COUNTAux_dec p np t nt ba  h (l0::ls) =
+     (COUNTAux_dec p np t t' ba h ([]: cand list) = T)
+  /\ (COUNTAux_dec p np t t' ba  (h: cand list) (l0::ls) =
        if (MEM l0 h) then
-        (get_cand_pile l0 np = (get_cand_pile l0 p) ++ FILTER (\ (b: (cand list) # rat). (fcc l0 (FST b) h)) ba)
-          /\ (get_cand_tally l0 nt = SUM_RAT (MAP SND (FILTER (\ (b: (cand list) # rat). (fcc l0 (FST b) h)) ba)))
-           /\ (COUNTAux_dec p np t nt ba h ls)
+        (get_cand_pile l0 np = (get_cand_pile l0 p) ++ FILTER (\ (b: (cand list) # rat). (first_continuing_cand_dec l0 (FST b) h)) ba)
+          /\ ((get_cand_tally l0 t') = SUM_RAT (MAP SND (FILTER (\ (b: (cand list) # rat). (first_continuing_cand_dec l0 (FST b) h)) ba))) 
+           /\ (COUNTAux_dec p np t t' ba h ls)
         else
              (get_cand_pile l0 np = get_cand_pile l0 p)
-          /\ (get_cand_tally l0 nt = get_cand_tally l0 t)
-          /\ (COUNTAux_dec p np t nt ba h ls))`;
+          /\ ((get_cand_tally l0 t') = get_cand_tally l0 t)
+          /\ (COUNTAux_dec p np t t' ba h ls))`;
 
-
- val COUNT_dec = Define `
-    (COUNT_dec st (qu : rat) (l: cand list) ((j: judgement), winners w) = F)
- /\ (COUNT_dec st qu l (winners w, (j: judgement)) = F)
- /\ (COUNT_dec st qu l (state (ba, t, p, bl, e, h), state (ba', t', p', bl', e',h')) =
-       (CountAux_dec p p' t t' ba h l)
-    /\ (bl = bl') /\ (e = e') /\ (h = h')
-    /\ (no_dup (h++e))
-    /\ no_dup (MAP FST p)
-    /\ (list_MEM (h++e) l)
-    /\ (Valid_PileTally_DEC1 t l) /\ (Valid_PileTally_DEC2 t l)
-    /\ (Valid_PileTally_DEC1 t' l) /\ (Valid_PileTally_DEC2 t' l)
-    /\ (Valid_PileTally_DEC1 p l) /\ (Valid_PileTally_DEC2 p l)
-    /\ (Valid_PileTally_DEC1 p' l) /\ (Valid_PileTally_DEC2 p' l)
-    /\ no_dup (MAP FST p')
-    /\ no_dup (MAP FST t')
-    /\ (non_empty l) /\ (no_dup l)
-    /\ (no_dup (MAP FST t))
-    /\ (non_empty ba)
-    /\ (non_empty h)
-    /\ (ba' = []))`;
-
-
-
+ 
 val Logical_to_Functional_Count_Dec_Aux = Q.store_thm ("Logical_to_Functional_Count_Dec_Aux",
  `!t nt p np ba h l.
           (!c. MEM c l ==>
@@ -961,7 +909,7 @@ val Logical_to_Functional_Count_Dec_Aux = Q.store_thm ("Logical_to_Functional_Co
                                       /\ (get_cand_tally c nt = get_cand_tally c t))))
                                            ==> COUNTAux_dec p np t nt ba h l`,
 
-
+ 
 Induct_on `l`
   >- rw[COUNTAux_dec]
   >- ((REPEAT STRIP_TAC
@@ -969,21 +917,19 @@ Induct_on `l`
 
     >- (first_assum (qspecl_then [`h`] strip_assume_tac)
      >> FULL_SIMP_TAC list_ss [MEM]
-      >> `!c h ba. first_continuing_cand c h ba <=> fcc c h ba`
+      >> `!c h ba. first_continuing_cand c h ba <=> first_continuing_cand_dec c h ba`
               by metis_tac [first_continuing_cand_IMP_fcc,fcc_to_first_continuing_cand]
          >> metis_tac [])
 
     >- (first_assum (qspecl_then [`h`] strip_assume_tac)
      >> FULL_SIMP_TAC list_ss []
-       >> `!c h ba. first_continuing_cand c h ba <=> fcc c h ba`
+       >> `!c h ba. first_continuing_cand c h ba <=> first_continuing_cand_dec c h ba`
               by metis_tac [first_continuing_cand_IMP_fcc,fcc_to_first_continuing_cand]
          >> metis_tac [])));
+ 
 
 
-
-
-
-
+  
 val Functional_to_Logical_Count_Dec_Aux = Q.store_thm ("Functional_to_Logical_Count_Dec_Aux",
 `!t nt p np ba h l. COUNTAux_dec p np t nt ba h l ==>
           (!c. MEM c l ==>
@@ -1001,124 +947,153 @@ Induct_on `l`
   >- rw[]
   >- (REPEAT STRIP_TAC
       >- (`(c = h) \/ (MEM c l)` by FULL_SIMP_TAC list_ss [MEM]
-           >- ((MAP_EVERY qexists_tac [`FILTER (\ (b: (cand list) # rat). (fcc c (FST b) h')) ba`]
-            >> `!c h ba. first_continuing_cand c h ba <=> fcc c h ba`
+           >- ((MAP_EVERY qexists_tac [`FILTER (\ (b: (cand list) # rat). (first_continuing_cand_dec c (FST b) h')) ba`]
+            >> `!c h ba. first_continuing_cand c h ba <=> first_continuing_cand_dec c h ba`
               by metis_tac [first_continuing_cand_IMP_fcc,fcc_to_first_continuing_cand]
               >>  STRIP_TAC)
                  >- metis_tac []
-                 >- metis_tac[CountAux_dec])
-           >- ((MAP_EVERY qexists_tac [`FILTER (\ (b: (cand list) # rat). (fcc c (FST b) h')) ba`]
-            >> `!c h ba. first_continuing_cand c h ba <=> fcc c h ba`
+                 >- metis_tac[COUNTAux_dec])
+           >- ((MAP_EVERY qexists_tac [`FILTER (\ (b: (cand list) # rat). (first_continuing_cand_dec c (FST b) h')) ba`]
+            >> `!c h ba. first_continuing_cand c h ba <=> first_continuing_cand_dec c h ba`
               by metis_tac [first_continuing_cand_IMP_fcc,fcc_to_first_continuing_cand]
               >> STRIP_TAC)
                 >- metis_tac []
                 >- metis_tac [COUNTAux_dec]))
-       >- metis_tac[CountAux_dec,MEM]
+       >- metis_tac[COUNTAux_dec,MEM]
        >- metis_tac [COUNTAux_dec,MEM]));
 
 
-
+  
 val intermediate_count_IMP_Count_Aux = Q.store_thm ("intermediate_count_IMP_Count_Aux",
- `! (st: num) (qu: rat) l j1 j2. intermediate_count st qu l j1 j2 ==> COUNT st qu l j1 j2`,
+ `! (st: num) (qu: rat) l j1 j2. intermediate_count (qu,st,l) j1 j2 ==> COUNT (qu,st,l) j1 j2`,
 
+  
+(REPEAT STRIP_TAC >> rw[COUNT_def] >> rfs[intermediate_count_def]      
+     >> STRIP_TAC)   
+     >- metis_tac[]   
+     >- (REPEAT STRIP_TAC     
 
-(REPEAT STRIP_TAC
-  >> rw[COUNT_def]
-    >> rfs[intermediate_count_def]
-      >> STRIP_TAC)
-  >- metis_tac []
-  >- (REPEAT STRIP_TAC
-     >- metis_tac [Valid_PileTally,PileTally_DEC2_IMP_PileTally,EVERY_CAND_HAS_ONE_PILE]
-     >- metis_tac [Valid_PileTally,PileTally_DEC2_IMP_PileTally,EVERY_CAND_HAS_ONE_TALLY]
-     >- (`get_cand_pile c np = get_cand_pile c p` by metis_tac []
-      >> `!L. MEM (c,L) np ==> (get_cand_pile c np = L)` by
-            metis_tac [Valid_PileTally,PileTally_DEC2_IMP_PileTally,EVERY_CAND_HAS_ONE_PILE]
-        >> `!L. MEM (c,L) p ==> (get_cand_pile c p = L)` by
-            metis_tac [Valid_PileTally,PileTally_DEC2_IMP_PileTally,EVERY_CAND_HAS_ONE_PILE]
-          >> `!L. MEM (c,L) p ==> MEM (c,L) np` by (REPEAT STRIP_TAC >>
-              metis_tac [Valid_PileTally,PileTally_DEC2_IMP_PileTally,GET_CAND_PILE_MEM])
+       >- metis_tac[Valid_PileTally_def,PileTally_DEC2_IMP_PileTally,EVERY_CAND_HAS_ONE_PILE]
+       >- (`!L. MEM (c,L) nt' ==> (get_cand_tally c nt' = L)` by
+            metis_tac [Valid_PileTally_def,PileTally_DEC2_IMP_PileTally,EVERY_CAND_HAS_ONE_TALLY]
+         >> `!L. MEM (c,L) t ==> (get_cand_tally c t = L)` by
+           metis_tac [Valid_PileTally_def,PileTally_DEC2_IMP_PileTally,EVERY_CAND_HAS_ONE_TALLY]
+	    >> metis_tac[])  
+       >- (`!L. MEM (c,L) np ==> (get_cand_pile c np = L)` by
+            metis_tac [Valid_PileTally_def,PileTally_DEC2_IMP_PileTally,EVERY_CAND_HAS_ONE_PILE]
+         >> `!L. MEM (c,L) p ==> (get_cand_pile c p = L)` by
+            metis_tac [Valid_PileTally_def,PileTally_DEC2_IMP_PileTally,EVERY_CAND_HAS_ONE_PILE]
+         >> `!L. MEM (c,L) p ==> MEM (c,L) np` by (REPEAT STRIP_TAC >>
+              metis_tac [Valid_PileTally_def,PileTally_DEC2_IMP_PileTally,GET_CAND_PILE_MEM])
             >> `!L. MEM (c,L) np ==> MEM (c,L) p` by (REPEAT STRIP_TAC >>
-                metis_tac [Valid_PileTally,PileTally_DEC2_IMP_PileTally,GET_CAND_PILE_MEM])
-              >> metis_tac [])
-     >- (`get_cand_tally c nt = get_cand_tally c t` by metis_tac []
-        >> `!L. MEM (c,L) nt ==> (get_cand_tally c nt = L)` by
-            metis_tac [Valid_PileTally,PileTally_DEC2_IMP_PileTally,EVERY_CAND_HAS_ONE_TALLY]
-          >> `!L. MEM (c,L) t ==> (get_cand_tally c t = L)` by
-              metis_tac [Valid_PileTally,PileTally_DEC2_IMP_PileTally,EVERY_CAND_HAS_ONE_TALLY]
-            >> `!L. MEM (c,L) t ==> MEM (c,L) nt` by (REPEAT STRIP_TAC >>
-                metis_tac [Valid_PileTally,PileTally_DEC2_IMP_PileTally,GET_CAND_TALLY_MEM2])
-             >> `!L. MEM (c,L) nt ==> MEM (c,L) t` by (REPEAT STRIP_TAC >>
-                 metis_tac [Valid_PileTally,PileTally_DEC2_IMP_PileTally,GET_CAND_TALLY_MEM2])
-               >> metis_tac [])));
-
-
-
+                 metis_tac [Valid_PileTally_def,PileTally_DEC2_IMP_PileTally,GET_CAND_PILE_MEM])
+              >> metis_tac []) 
+        >- (`!L. MEM (c,L) nt' ==> (get_cand_tally c nt' = L)` by
+            metis_tac [Valid_PileTally_def,PileTally_DEC2_IMP_PileTally,EVERY_CAND_HAS_ONE_TALLY]
+         >> `!L. MEM (c,L) t ==> (get_cand_tally c t = L)` by
+           metis_tac [Valid_PileTally_def,PileTally_DEC2_IMP_PileTally,EVERY_CAND_HAS_ONE_TALLY]
+         >> `!L. MEM (c,L) t ==> MEM (c,L) nt'` by (REPEAT STRIP_TAC >>
+              metis_tac [Valid_PileTally_def,PileTally_DEC2_IMP_PileTally,GET_CAND_TALLY_MEM2])
+            >> `!L. MEM (c,L) nt' ==> MEM (c,L) t` by (REPEAT STRIP_TAC >>
+                 metis_tac [Valid_PileTally_def,PileTally_DEC2_IMP_PileTally,GET_CAND_TALLY_MEM2])
+              >> metis_tac []))); 
+               
+   
+  
+    
 val Count_Aux_IMP_intermediate_count = Q.store_thm ("Count_Aux_IMP_intermediate_count",
-`! (st: num) (qu: rat) l j1 j2. COUNT st qu l j1 j2 ==> intermediate_count st qu l j1 j2`,
+`! (st: num) (qu: rat) l j1 j2. COUNT (qu,st,l) j1 j2 ==> intermediate_count (qu,st,l) j1 j2`,
 
-(REPEAT STRIP_TAC
+(REPEAT STRIP_TAC 
  >> rw[intermediate_count_def]
   >> rfs[COUNT_def]
-   >> STRIP_TAC)
-   >- metis_tac[]
-   >- (REPEAT STRIP_TAC
+   >> STRIP_TAC)  
+   >- metis_tac[] 
+   >- (REPEAT STRIP_TAC 
      >- (`(!l'. MEM (c,l') np ==>
-       (l' = (get_cand_pile c p) ++ (FILTER (\ (b: (Cand list) # rat).(first_continuing_cand c (FST b) h)) ba)))`
+       (l' = (get_cand_pile c p) ++ (FILTER (\ (b: (cand list) # rat).(first_continuing_cand c (FST b) h)) ba)))`
         by  metis_tac[]
       >> first_assum (qspecl_then [`get_cand_pile c np`] strip_assume_tac)
-        >> metis_tac [Valid_PileTally,PileTally_DEC2_IMP_PileTally,GET_CAND_PILE_MEM])
-     >- metis_tac [Valid_PileTally,PileTally_DEC2_IMP_PileTally,GET_CAND_TALLY_MEM2]
+        >> metis_tac [Valid_PileTally_def,PileTally_DEC2_IMP_PileTally,GET_CAND_PILE_MEM])
+     >- metis_tac [Valid_PileTally_def,PileTally_DEC2_IMP_PileTally,GET_CAND_TALLY_MEM2]
      >- (`(!l'. MEM c l /\ MEM (c,l') np <=> MEM c l /\ MEM (c,l') p)` by metis_tac []
        >> `MEM (c,get_cand_pile c np) p` by
-           metis_tac [Valid_PileTally,PileTally_DEC2_IMP_PileTally,GET_CAND_PILE_MEM,EVERY_CAND_HAS_ONE_PILE]
-         >> metis_tac [Valid_PileTally,PileTally_DEC2_IMP_PileTally,EVERY_CAND_HAS_ONE_PILE])
-     >- (`(!r. MEM c l /\ MEM (c,r) t <=> MEM c l /\ MEM (c,r) nt) ` by metis_tac []
-      >> metis_tac [Valid_PileTally,PileTally_DEC2_IMP_PileTally,EVERY_CAND_HAS_ONE_TALLY,GET_CAND_TALLY_MEM2])));
+           metis_tac [Valid_PileTally_def,PileTally_DEC2_IMP_PileTally,GET_CAND_PILE_MEM,EVERY_CAND_HAS_ONE_PILE]
+         >> metis_tac [Valid_PileTally_def,PileTally_DEC2_IMP_PileTally,EVERY_CAND_HAS_ONE_PILE])
+     >- (`(!r. MEM c l /\ MEM (c,r) t <=> MEM c l /\ MEM (c,r) nt') ` by metis_tac []
+      >> metis_tac [Valid_PileTally_def,PileTally_DEC2_IMP_PileTally,EVERY_CAND_HAS_ONE_TALLY,GET_CAND_TALLY_MEM2])));
+  
+ 
 
 
 
-
-
+(* to be reconstructed
 
 val Count_Aux_IMP_Count_Aux_dec = Q.store_thm ("Count_Aux_IMP_Count_Aux_dec",
- `! (st: num) (qu: rat) l j1 j2. COUNT st qu l j1 j2 ==> COUNT_dec st qu l (j1,j2)`,
+ `! (st: num) (qu: rat) l j1 j2. COUNT (qu,st,l) j1 j2 ==> COUNT_dec (qu,st,l) j1 j2`,
 
-  (ASSUME_TAC Count_Aux_IMP_intermediate_count
-   >> REPEAT STRIP_TAC
-    >> `intermediate_count st qu l j1 j2` by metis_tac[COUNT_def,Count_Aux_IMP_intermediate_count]
-     >> rfs[COUNT_dec,COUNT_def]
+  (ASSUME_TAC Count_Aux_IMP_intermediate_count 
+   >> REPEAT STRIP_TAC 
+   >> `intermediate_count (qu,st,l) j1 j2` by metis_tac[COUNT_def,Count_Aux_IMP_intermediate_count]
+     >> rfs[COUNT_dec_def,COUNT_def] 
       >> REPEAT STRIP_TAC)
-        >- (rfs [intermediate_count_def]
-         >> metis_tac [ Logical_to_Functional_Count_Dec_Aux])
-        >- metis_tac[NO_DUP_PRED_to_no_dup]
-        >- metis_tac[NO_DUP_PRED_to_no_dup]
+        >-  (rfs [intermediate_count_def]  
+         ASSUME_TAC Logical_to_Functional_Count_Dec_Aux	
+        first_assum (qspecl_then [`t`,`nt'`,`p`,`np`,`ba`,`h`,`l`] strip_assume_tac)
+        `!c. MEM c l ==>
+	      (MEM c h ==>
+	               ?l. (l = FILTER (λb. first_continuing_cand c (FST b) h) ba) /\
+		       (get_cand_pile c np = (get_cand_pile c p) ++ l) /\
+		       (get_cand_tally c nt' = SUM_RAT (MAP SND l)))
+	  /\  ((~ MEM c h) ==>
+	               (get_cand_pile c np = get_cand_pile c p) /\
+		       (get_cand_tally c nt' = get_cand_tally c t))`
+		       by (REPEAT STRIP_TAC
+                      >- (MAP_EVERY qexists_tac [`FILTER (λb. first_continuing_cand c (FST b) h) ba`]
+		        >> fs[])
+                      >- metis_tac[] 
+                      >- metis_tac[]) 
+         metis_tac simp_tac bool_ss fs[COUNTAux_dec_def, Logical_to_Functional_Count_Dec_Aux] 		         UNDISCH_TAC [`!c. MEM c l ==>
+	      (MEM c h ==>
+	               ?l. (l = FILTER (λb. first_continuing_cand c (FST b) h) ba) /\
+		       (get_cand_pile c np = (get_cand_pile c p) ++ l) /\
+		       (get_cand_tally c nt' = SUM_RAT (MAP SND l)))
+	  /\  ((~ MEM c h) ==>
+	               (get_cand_pile c np = get_cand_pile c p) /\
+		       (get_cand_tally c nt' = get_cand_tally c t))`]
+	     	       
+   
+
+>- metis_tac[] 
+        >- metis_tac[]
         >- metis_tac [Logical_list_MEM_VICE_VERCA_TheFunctional,MEM_APPEND]
-        >- metis_tac [Valid_PileTally,PileTally_to_PileTally_DEC1]
-        >- metis_tac [Valid_PileTally,PileTally_to_PileTally_DEC2]
-        >- metis_tac [Valid_PileTally,PileTally_to_PileTally_DEC1]
-        >- metis_tac [Valid_PileTally,PileTally_to_PileTally_DEC2]
-        >- metis_tac [Valid_PileTally,PileTally_to_PileTally_DEC1]
-        >- metis_tac [Valid_PileTally,PileTally_to_PileTally_DEC2]
-        >- metis_tac [Valid_PileTally,PileTally_to_PileTally_DEC1]
-        >- metis_tac [Valid_PileTally,PileTally_to_PileTally_DEC2]
-        >- metis_tac [NO_DUP_PRED_to_no_dup]
-        >- metis_tac [NO_DUP_PRED_to_no_dup]
-        >- (`l <> []` by metis_tac[Valid_Init_CandList]
+        >- metis_tac [Valid_PileTally_def,PileTally_to_PileTally_DEC1]
+        >- metis_tac [Valid_PileTally_def,PileTally_to_PileTally_DEC2]
+        >- metis_tac [Valid_PileTally_def,PileTally_to_PileTally_DEC1]
+        >- metis_tac [Valid_PileTally_def,PileTally_to_PileTally_DEC2]
+        >- metis_tac [Valid_PileTally_def,PileTally_to_PileTally_DEC1]
+        >- metis_tac [Valid_PileTally_def,PileTally_to_PileTally_DEC2]
+        >- metis_tac [Valid_PileTally_def,PileTally_to_PileTally_DEC1]
+        >- metis_tac [Valid_PileTally_def,PileTally_to_PileTally_DEC2]
+        >- metis_tac []
+        >- metis_tac []
+        >- (`l <> []` by metis_tac[Valid_Init_CandList_def]
          >> `?l1 x. l = x::l1` by metis_tac [list_nchotomy]
-           >> rw[non_empty])
-        >- metis_tac [Valid_Init_CandList,NO_DUP_PRED_to_no_dup]
-        >- metis_tac [NO_DUP_PRED_to_no_dup]
-        >- (`? X BA. ba = X::BA` by metis_tac [list_nchotomy] >> rw[non_empty])
-        >- (`? h0 hs. h = h0::hs` by metis_tac [list_nchotomy] >> rw[non_empty]));
-
-
+           >> fs[NULL])
+        >- metis_tac [Valid_Init_CandList_def]
+        >- metis_tac []
+        >- (`? X BA. ba = X::BA` by metis_tac [list_nchotomy] >> fs[NULL])
+        >- (`? h0 hs. h = h0::hs` by metis_tac [list_nchotomy] >> fs[NULL]));
+*)
+ 
+(* to be reconstructed
 
 val Count_Aux_dec_IMP_Count_Aux = Q.store_thm ("Count_Aux_dec_IMP_Count_Aux",
- `! (st : num) (qu:rat) l j1 j2. COUNT_dec st qu l (j1,j2) ==> COUNT st qu l j1 j2 `,
+ `! (st : num) (qu:rat) l j1 j2. COUNT_dec (qu,st,l) j1 j2 ==> COUNT (qu,st,l) j1 j2 `,
 
  (ASSUME_TAC intermediate_count_IMP_Count_Aux
-  >> REPEAT STRIP_TAC
-    >> `intermediate_count st qu l j1 j2` by
+  >> REPEAT STRIP_TAC 
+    >> `intermediate_count (qu,st,l) j1 j2` by
       (Cases_on `j1`
        >- (Cases_on `j2`
          >- ((Cases_on `p` >> Cases_on `r` >> Cases_on `r'` >> Cases_on `r` >> Cases_on `r'`
@@ -1149,9 +1124,9 @@ val Count_Aux_dec_IMP_Count_Aux = Q.store_thm ("Count_Aux_dec_IMP_Count_Aux",
          >- rfs [COUNT_dec])
         >- (Cases_on `j2`
          >- rfs [COUNT_dec]
-         >- rfs [COUNT_dec])))
+         >- rfs [COUNT_dec]))
            >> metis_tac[]);
-
+*)
 
 
 val APPEND_EQ_NIL2 = Q.store_thm ("APPEND_EQ_NIL2",
@@ -1163,149 +1138,135 @@ val APPEND_EQ_NIL2 = Q.store_thm ("APPEND_EQ_NIL2",
             >> (ASM_SIMP_TAC bool_ss [NOT_NIL_CONS]
               >> STRIP_TAC
                 >> rw[NOT_NIL_CONS]))) ;
-
-
+ 
+ 
 val take_append_returns_appended = Q.store_thm ("take_append_returns_appended",
  `! l1 l2 l3. (l1 = l2 ++ l3) ==> (l3 = take_append l1 l2)`,
 
  Induct_on `l1`
-  >- FULL_SIMP_TAC list_ss [APPEND_EQ_NIL2,take_append]
+  >- FULL_SIMP_TAC list_ss [APPEND_EQ_NIL2,take_append_def]
   >- (Induct_on `l2`
-    >- FULL_SIMP_TAC list_ss [APPEND_NIL_LEFT,take_append]
+    >- FULL_SIMP_TAC list_ss [APPEND_NIL_LEFT,take_append_def]
     >- (REPEAT STRIP_TAC
-     >> rw[take_append]
+     >> rw[take_append_def]
        >> FULL_SIMP_TAC list_ss [CONS_11])));
-
-
+ 
+  
 val eqe_list_dec_MEM1 = Q.store_thm ("list_eqe_dec_MEM1",
  `!l0 l1 l2. eqe_list_dec l0 l1 l2 ==> (!c. MEM c l0 \/ MEM c l1 ==> MEM c l2)`,
-
+ 
 Induct_on `l0`
-  >- metis_tac [eqe_list_dec,list_MEM_def,Logical_list_MEM_VICE_VERCA_TheFunctional]
+  >- fs [eqe_list_dec_def,Logical_list_MEM_VICE_VERCA_TheFunctional]     
   >- (REPEAT STRIP_TAC
-     >- metis_tac [eqe_list_dec,MEM]
-     >- metis_tac [MEM,eqe_list_dec]));
-
-
+     >- metis_tac [eqe_list_dec_def,MEM]
+     >- metis_tac [MEM,eqe_list_dec_def]));
+   
+    
 val logical_to_functional_eqe_list_dec = Q.store_thm ("logical_to_functional_eqe_list_dec",
-`!l0 l1 l2. (!c. NO_DUP_PRED (l0 ++ l1) c) /\ (!c. MEM c l0 \/ MEM c l1 ==> MEM c l2) ==> eqe_list_dec l0 l1 l2`,
-
+`!l0 l1 l2. (ALL_DISTINCT (l0 ++ l1)) /\ (!c. MEM c l0 \/ MEM c l1 ==> MEM c l2) ==> eqe_list_dec l0 l1 l2`,
+  
    Induct_on `l0`
-     >- metis_tac [eqe_list_dec,list_MEM_def,Logical_list_MEM_VICE_VERCA_TheFunctional]
-     >- ((REPEAT STRIP_TAC
-       >> rw[eqe_list_dec])
-           >- (`no_dup (h::l0 ++ l1)` by metis_tac [NO_DUP_PRED_to_no_dup]
-             >> `!G1 G2 (s: Cand). (not_elem s (G1++G2) = (not_elem s G1) /\ (not_elem s G2))`
-                             by (Induct_on `G1`
-                              >- FULL_SIMP_TAC list_ss [APPEND_NIL_LEFT,not_elem]
-                              >- ((ASSUME_TAC CAND_EQ_DEC >> REPEAT STRIP_TAC
-                                >> first_x_assum (qspecl_then [`s`,`h'`] strip_assume_tac))
-                                 >- FULL_SIMP_TAC list_ss [not_elem]
-                                 >- FULL_SIMP_TAC list_ss [not_elem]))
-                >> FULL_SIMP_TAC list_ss [no_dup,not_elem,not_elem_NOT_MEM])
-           >- (FULL_SIMP_TAC list_ss [NO_DUP_TAIL_ONE_CAND,MEM] >> metis_tac [NO_DUP_TAIL_ONE_CAND,MEM])));
-
-
-
-
-val eqe_list_dec2 = Define `
-     (eqe_list_dec2 l0 l1 ([]: Cand list) = T)
-  /\ (eqe_list_dec2 l0 l1 (l::ls) = (MEM l l0 \/ MEM l l1) /\ (eqe_list_dec2 l0 l1 ls))`;
-
+     >- metis_tac [eqe_list_dec_def,Logical_list_MEM_VICE_VERCA_TheFunctional]
+     >-  ((REPEAT STRIP_TAC  
+       >> rw[eqe_list_dec_def])
+          >- fs [ALL_DISTINCT]
+          >- (`!c. MEM c l0 \/ MEM c l1 ==> MEM c l2` by metis_tac[MEM]
+	    >> `ALL_DISTINCT (l0 ++ l1)` by fs[ALL_DISTINCT] 
+              >> metis_tac[ALL_DISTINCT,MEM])));  
+  
 
 val eqe_list_dec2_verified = Q.store_thm ("eqe_list_dec2_verified",
  `! l0 l1 l2. eqe_list_dec2 l0 l1 l2 <=> (!c. MEM c l2 ==> MEM c l0 \/ MEM c l1)`,
   Induct_on `l2`
-    >- rw[eqe_list_dec2]
-    >- (REPEAT STRIP_TAC
-    >> metis_tac [MEM,eqe_list_dec2]));
-
-
+    >-  (EVAL_TAC >> rw[])            
+    >- (REPEAT STRIP_TAC >> rfs[]   
+        >> fs[eqe_list_dec2_def]  
+        >> metis_tac[eqe_list_dec2_def]));
+  
 val functional_to_logical_BiggerThanQuota = Q.store_thm ("logical_to_functional_BiggerThanQuota",
- `! (qu:rat) l t. bigger_than_quota l t qu /\ no_dup (MAP FST t) ==>
+ `! (qu:rat) l t. bigger_than_quota l t qu /\ ALL_DISTINCT (MAP FST t) ==>
                                      (!c. MEM c l ==> (!r. MEM (c,r) t ==> qu <= r))`,
-
+ 
   Induct_on `l`
-    >- rw[]
-    >- ((REPEAT STRIP_TAC
+    >- rw[] 
+    >- ((REPEAT STRIP_TAC 
       >> FULL_SIMP_TAC list_ss [])
-         >- (`get_cand_tally c t = r` by metis_tac [no_dup_IMP_NO_DUP_PRED,EVERY_CAND_HAS_ONE_TALLY]
-           >> metis_tac [RAT_LEQ_REF,bigger_than_quota])
-         >- metis_tac [bigger_than_quota]));
+         >- (`get_cand_tally c t = r` by metis_tac [ALL_DISTINCT,EVERY_CAND_HAS_ONE_TALLY] 
+           >> RW_TAC bool_ss [] >> rfs[bigger_than_quota_def])   
+         >- (`bigger_than_quota l t qu` by fs[bigger_than_quota_def] 
+	    >> metis_tac [])));  
+     
 
-
-
+    
 val logical_to_functional_BiggerThanQuota = Q.store_thm ("logical_to_functional_BiggerThanQuota",
-`! (qu: rat) l t. (!c. NO_DUP_PRED (MAP FST t) c) /\ (!d. MEM d l ==> MEM d (MAP FST t)) /\
+`! (qu: rat) l t. (ALL_DISTINCT (MAP FST t)) /\ (!d. MEM d l ==> MEM d (MAP FST t)) /\
                   (!c. MEM c l ==> (!r. MEM (c,r) t ==> qu <= r)) ==> bigger_than_quota l t qu`,
-
+ 
   Induct_on `l`
-     >- rw[bigger_than_quota]
+     >- rw[bigger_than_quota_def] 
      >- ((REPEAT STRIP_TAC
-       >> rw[bigger_than_quota])
+       >> rw[bigger_than_quota_def]) 
           >- (`MEM (h,get_cand_tally h t) t` by metis_tac [MEM,GET_CAND_TALLY_MEM2]
             >> metis_tac[MEM])
-          >- metis_tac [MEM]));
-
-
+          >- metis_tac [bigger_than_quota_def,MEM]));
+ 
+   
 val functional_to_logicl_piles_eq = Q.store_thm ("functional_to_logical_piles_eq",
- `! l1 l2 p1 p2. no_dup (MAP FST p1) /\ no_dup (MAP FST p2) /\ (list_MEM l1 (MAP FST p1)) /\
+ `! l1 l2 p1 p2. ALL_DISTINCT (MAP FST p1) /\ ALL_DISTINCT (MAP FST p2) /\ (list_MEM l1 (MAP FST p1)) /\
                 (list_MEM l1 (MAP FST p2)) /\ (piles_eq_list l1 l2 p1 p2) ==>
    (!c. MEM c l1 ==> (~ MEM c l2 ==> (!l'. MEM (c,l') p1 <=> MEM (c,l') p2)))`,
 
 Induct_on `l1`
  >- rw[]
-
+  
  >- ((REPEAT STRIP_TAC
-    >> FULL_SIMP_TAC list_ss [])
-
-  >- (`get_cand_pile h p1 = get_cand_pile h p2` by metis_tac [piles_eq_list] >>
+    >> Cases_on `c= h`)
+      
+  >- (`get_cand_pile h p1 = get_cand_pile h p2` by metis_tac [piles_eq_list_def] >>
      (`MEM (h,l') p1 ==> MEM (h, l') p2` by (STRIP_TAC >>
      `get_cand_pile c p1 = l'` by
-     metis_tac [Logical_list_MEM_VICE_VERCA_TheFunctional,MEM,list_MEM_def,no_dup_IMP_NO_DUP_PRED,
+     metis_tac [Logical_list_MEM_VICE_VERCA_TheFunctional,MEM,
      GET_CAND_PILE_MEM,EVERY_CAND_HAS_ONE_PILE] >>
        `MEM (h,get_cand_pile h p2) p2` by
-       metis_tac [Logical_list_MEM_VICE_VERCA_TheFunctional,MEM,list_MEM_def,no_dup_IMP_NO_DUP_PRED,
+       metis_tac [Logical_list_MEM_VICE_VERCA_TheFunctional,MEM,
        GET_CAND_PILE_MEM,EVERY_CAND_HAS_ONE_PILE] >>
          `l' = get_cand_pile h p2` by
-         metis_tac [Logical_list_MEM_VICE_VERCA_TheFunctional,MEM,list_MEM_def,no_dup_IMP_NO_DUP_PRED,
+         metis_tac [Logical_list_MEM_VICE_VERCA_TheFunctional,MEM,
          GET_CAND_PILE_MEM,EVERY_CAND_HAS_ONE_PILE] >>
-           metis_tac [MEM])) >>
+           metis_tac [MEM])) >> 
      (`MEM (h,l') p2 ==> MEM (h,l') p1` by (STRIP_TAC >>
      `get_cand_pile c p2 = l'`
-     by metis_tac [Logical_list_MEM_VICE_VERCA_TheFunctional,MEM,list_MEM_def,no_dup_IMP_NO_DUP_PRED,
+     by metis_tac [Logical_list_MEM_VICE_VERCA_TheFunctional,MEM,
      GET_CAND_PILE_MEM,EVERY_CAND_HAS_ONE_PILE] >>
        `MEM (h,get_cand_pile h p1) p1` by
-       metis_tac [Logical_list_MEM_VICE_VERCA_TheFunctional,MEM,list_MEM_def,no_dup_IMP_NO_DUP_PRED,
+       metis_tac [Logical_list_MEM_VICE_VERCA_TheFunctional,MEM,
        GET_CAND_PILE_MEM,EVERY_CAND_HAS_ONE_PILE] >>
          `l' = get_cand_pile h p1` by
-         metis_tac [Logical_list_MEM_VICE_VERCA_TheFunctional,MEM,list_MEM_def,no_dup_IMP_NO_DUP_PRED,
+         metis_tac [Logical_list_MEM_VICE_VERCA_TheFunctional,MEM,
          GET_CAND_PILE_MEM,EVERY_CAND_HAS_ONE_PILE] >>
-            metis_tac [MEM])) >>
+            metis_tac [MEM])) >> 
      metis_tac [MEM])
-
-
-   >- (`list_MEM l1 (MAP FST p1)` by metis_tac [MEM,list_MEM_def,Logical_list_MEM_VICE_VERCA_TheFunctional] >>
-      `list_MEM l1 (MAP FST p2)` by metis_tac [MEM,list_MEM_def,Logical_list_MEM_VICE_VERCA_TheFunctional] >>
-      `piles_eq_list l1 l2 p1 p2` by metis_tac [piles_eq_list] >>
+  >- (`list_MEM l1 (MAP FST p1)` by metis_tac [MEM,Logical_list_MEM_VICE_VERCA_TheFunctional] >>
+      `list_MEM l1 (MAP FST p2)` by metis_tac [MEM,Logical_list_MEM_VICE_VERCA_TheFunctional] >>
+      `piles_eq_list l1 l2 p1 p2` by metis_tac [piles_eq_list_def] >> 
       metis_tac [MEM])));
-
+   
 
 val logical_to_functional_piles_eq = Q.store_thm ("logical_to_functional_piles_eq",
 `! l1 l2 p1 p2.  (!c. MEM c l1 ==> (~ MEM c l2 ==> (!l'. MEM (c,l') p1 <=> MEM (c,l') p2)))
-              /\ (!c. NO_DUP_PRED (MAP FST p1) c) /\ (!c. NO_DUP_PRED (MAP FST p2) c)
+              /\ (ALL_DISTINCT (MAP FST p1)) /\ (ALL_DISTINCT (MAP FST p2) )
               /\ (!d. MEM d l1 ==> MEM d (MAP FST p1) /\ MEM d (MAP FST p2)) ==> piles_eq_list l1 l2 p1 p2`,
 
   Induct_on `l1`
-    >- rw[piles_eq_list]
+    >- rw[piles_eq_list_def]
     >- (REPEAT STRIP_TAC
-     >> rw[piles_eq_list]
+     >> rw[piles_eq_list_def]
       >> `!l'. MEM (h,l') p1 <=> MEM (h,l') p2` by FULL_SIMP_TAC list_ss [MEM]
        >> metis_tac [GET_CAND_PILE_MEM,EVERY_CAND_HAS_ONE_PILE,MEM]));
-
-
+ 
+ 
 val functional_to_logical_update_pile = Q.store_thm ("functional_to_logical_update_pile",
- `! (qu: rat) (t: (Cand # rat) list) l p1 p2. (!c. NO_DUP_PRED (MAP FST p1) c) /\ (!c. NO_DUP_PRED (MAP FST p2) c)
+ `! (qu: rat) (t: (cand # rat) list) l p1 p2. (ALL_DISTINCT (MAP FST p1)) /\ (ALL_DISTINCT (MAP FST p2))
         /\   (update_cand_pile qu t l p1 p2) ==>
               (!c. MEM c l ==> (!l'. MEM (c,l') p2 ==>
                                          (MAP FST l' = MAP FST (get_cand_pile c p1))
@@ -1319,39 +1280,39 @@ val functional_to_logical_update_pile = Q.store_thm ("functional_to_logical_upda
            >> `MAP FST p2 = (MAP FST l1) ++ c :: (MAP FST l2)` by FULL_SIMP_TAC list_ss [FST,MAP_APPEND_TRIO]
             >> `MEM c (MAP FST p2)` by FULL_SIMP_TAC list_ss [MEM_APPEND]
              >> `l' = get_cand_pile h p2` by metis_tac [GET_CAND_PILE_MEM,EVERY_CAND_HAS_ONE_PILE]
-              >> metis_tac [update_cand_pile])
-          >- metis_tac [update_cand_pile])
+              >> metis_tac [update_cand_pile_def])
+          >- metis_tac [update_cand_pile_def])
        >- (FULL_SIMP_TAC list_ss []
          >- (`? l1 l2. p2 = l1 ++ (c,l') ::l2` by metis_tac [MEM,MEM_SPLIT]
           >> `MAP FST p2 = (MAP FST l1) ++ c :: (MAP FST l2)` by FULL_SIMP_TAC list_ss [FST,MAP_APPEND_TRIO]
            >> `MEM c (MAP FST p2)` by FULL_SIMP_TAC list_ss [MEM_APPEND]
             >> `l' = get_cand_pile h p2` by metis_tac [GET_CAND_PILE_MEM,EVERY_CAND_HAS_ONE_PILE]
-             >> metis_tac[update_cand_pile])
-       >- metis_tac [update_cand_pile])));
+             >> metis_tac[update_cand_pile_def])
+       >- metis_tac [update_cand_pile_def])));
 
 
-
+ 
 val logical_to_functional_update_pile = Q.store_thm ("logical_to_functional_update_pile",
- `! (qu: rat) (t: (Cand #rat) list) l p1 p2. (!c. MEM c l ==> MEM c (MAP FST p2)) /\
+ `! (qu: rat) (t: (cand #rat) list) l p1 p2. (!c. MEM c l ==> MEM c (MAP FST p2)) /\
                                             (!c. MEM c l ==> (!l'. MEM (c,l') p2 ==>
                                               (MAP FST l' = MAP FST (get_cand_pile c p1))
                                                 /\ (MAP SND l' = update_cand_trans_val qu c t p1))) ==>
                                                     (update_cand_pile qu t l p1 p2)`,
 
     Induct_on `l`
-      >- rw [update_cand_pile]
+      >- rw [update_cand_pile_def]
       >- ((REPEAT STRIP_TAC
-       >> rw[update_cand_pile])
+       >> rw[update_cand_pile_def])
           >- (`MEM (h,get_cand_pile h p2) p2` by metis_tac [MEM,GET_CAND_PILE_MEM]
             >> metis_tac [MEM])
           >- (`MEM (h,get_cand_pile h p2) p2` by metis_tac [MEM,GET_CAND_PILE_MEM]
             >> metis_tac [MEM])));
-
-
+ 
+ 
 val tally_comparison_total = Q.store_thm ("tally_comparison_total",
  `!t c1 c2. ((tally_comparison t) c1 c2) \/ ((tally_comparison t) c2 c1)`,
   ((REPEAT STRIP_TAC
-    >> rw[tally_comparison]
+    >> rw[tally_comparison_def]
      >> ASSUME_TAC RAT_LES_TOTAL
       >> first_assum (qspecl_then [`get_cand_tally c1 t`,`get_cand_tally c2 t`] strip_assume_tac))
          >- (DISJ1_TAC
@@ -1360,27 +1321,28 @@ val tally_comparison_total = Q.store_thm ("tally_comparison_total",
           >> metis_tac [RAT_LEQ_REF])
          >- (DISJ2_TAC
           >> metis_tac [RAT_LES_IMP_LEQ])));
-
-
+ 
+ 
 val tally_comparison_total_COR = Q.store_thm ("tally_comparison_total_COR",
  `!t. total (tally_comparison t)`,
 
-   (ASSUME_TAC (INST_TYPE [alpha |-> ``:Cand``] total_def)
+   (ASSUME_TAC (INST_TYPE [alpha |-> ``:cand``] total_def)
      >> STRIP_TAC
        >> first_assum (qspecl_then [`tally_comparison t`] strip_assume_tac)
          >> metis_tac [tally_comparison_total]));
+ 
 
-
-
+ 
 val tally_comparison_trans = Q.store_thm ("tally_comparison_trans",
  `!t. transitive (tally_comparison t)`,
 
    (STRIP_TAC
      >> `! c1 c2 c3. (tally_comparison t) c1 c2 /\ (tally_comparison t) c2 c3 ==> (tally_comparison t) c1 c3`
        by (REPEAT STRIP_TAC
-        >> metis_tac [tally_comparison,RAT_LEQ_TRANS])
+        >> metis_tac [tally_comparison_def,RAT_LEQ_TRANS])
           >> metis_tac[transitive_def]));
-
+ 
+(* to be constructed
 
 val Logical_to_Functional_elect = Q.store_thm ("Logical_to_Functional_elect",
  `! st (qu: rat) l j1 j2. elect st qu l j1 j2 ==> Elect_dec st qu l (j1,j2)`,
@@ -1424,7 +1386,9 @@ val Logical_to_Functional_elect = Q.store_thm ("Logical_to_Functional_elect",
          >> `(!c. MEM c l ==> MEM c (MAP FST p))` by metis_tac [MEM,Valid_PileTally]
            >> metis_tac [logical_to_functional_update_pile]));
 
+*)
 
+(* to be reconstructed 
 
 
 val Functional_to_Logical_elect = Q.store_thm ("Functional_to_Logical_elect",
@@ -1484,57 +1448,35 @@ val Functional_to_Logical_elect = Q.store_thm ("Functional_to_Logical_elect",
    >- rfs [Elect_dec]
    >- rfs [Elect_dec]));
 
-
-val All_elem_zero_verified = Q.store_thm ("All_elem_zero_verified",
- `! t. (!c. MEM c t ==> (c = rat_0)) <=> all_elem_zero t`,
-
-  Induct_on `t`
-     >- rw[all_elem_zero]
-     >- (REPEAT STRIP_TAC
-       >> metis_tac [all_elem_zero,MEM]));
-
-
-val All_elem_nil_verified = Q.store_thm ("All_elem_nil_verified",
- `! p. (!c. MEM c p ==> (c = [])) <=> all_elem_nil p`,
-
-  Induct_on `p`
-   >- rw[all_elem_nil]
-   >- (REPEAT STRIP_TAC
-     >> metis_tac [MEM,all_elem_nil]));
-
-
+*)
+ 
 val Initial_Judgement_IMP_TheLogical = Q.store_thm ("Initial_Judgement_IMP_TheLogical",
  `! l j. Initial_Judgement_dec l j ==> initial_judgement l j`,
 
-  (REPEAT STRIP_TAC >> rw[initial_judgement]
-    >> Cases_on `j`)
-
-     >- (Cases_on `p` >> Cases_on `r` >> Cases_on `r'` >> Cases_on `r` >> Cases_on `r'`
-      >> rfs [Initial_Judgement_dec]
-        >> metis_tac [All_elem_zero_verified,All_elem_nil_verified])
-     >- rfs[Initial_Judgement_dec]);
-
-
+  (REPEAT STRIP_TAC >> rw[initial_judgement_def] 
+    >> Cases_on `j`) 
+   
+     >- (PairCases_on `p` 
+        >> MAP_EVERY qexists_tac [`p0`,`p1`,`p2`]
+           >>  rfs[Initial_Judgement_dec_def,EVERY_MEM]    
+             >>  metis_tac[NULL_EQ]) 
+     >- metis_tac[Initial_Judgement_dec_def]); 
+      
+ 
 val Logical_to_Functional_Initial_Judgement = Q.store_thm ("Logical_to_Functional_Initial_Judgement",
  `! l j. initial_judgement l j ==> Initial_Judgement_dec l j`,
 
   (REPEAT STRIP_TAC
-    >> rfs [initial_judgement]
-      >> rw[Initial_Judgement_dec])
-         >- metis_tac [All_elem_zero_verified]
-         >- metis_tac [All_elem_nil_verified]);
+    >> rfs [initial_judgement_def]
+      >> rw[Initial_Judgement_dec_def])
+         >- FULL_SIMP_TAC list_ss [EVERY_MEM]   
+         >- FULL_SIMP_TAC list_ss [EVERY_MEM]);
+ 
 
-
-
-val Final_Judgement_dec = Define `
-           (Final_Judgement_dec (state (ba,t,p,bl,e,h)) = F)
-        /\ (Final_Judgement_dec (winners l) = T)`;
-
-
-
+(*
 val Elim_dec = Define `
          (Elim_dec st qu l (j1,j2) c = Elim_cand_dec st qu l c (j1,j2))`;
-
+ 
 
 
 val Checker_Aux_dec = Define `
@@ -1550,6 +1492,10 @@ val Checker_Aux_dec = Define `
                       \/ (EXISTS (Elim_dec st qu l (j0,HD js)) l))
                       /\ (Checker_Aux_dec st qu l js))`;
 
+
+*)
+
+(*
 val Logical_to_computational_checker= Q.store_thm("Logical_to_computatonal_checker",
  `! st qu l J. valid_judgement st qu l J ==> CHECKER_AUX_dec st qu l J`,
 
@@ -1599,5 +1545,7 @@ val Logical_to_computational_checker= Q.store_thm("Logical_to_computatonal_check
                    >> `h::j'::J' = h::J0 ++ [j0;j1] ++J1` by FULL_SIMP_TAC list_ss[]
                      >> metis_tac [])
                        >> metis_tac []))));
+
+*)
 
 val _ = export_theory();
